right_lemma completed

reduction_directedHamiltonianCircuit_to_hamiltonianCircuit/reduction_hamiltonian_rCompletness.dfy
@@ -1,10 +1,12 @@
 include "reduction_hamiltonian_definitions.dfy"
 include "reduction_hamiltonian_rFunction.dfy"
+include "permutation_property.dfy"
 
 module ReductionCompletness
 {
     import opened Definitions
     import opened ReductionFunction
+    import opened PermutationProperty
 
     ///// REDUCTION COMPLETNESS /////
 
@@ -34,87 +36,11 @@ module ReductionCompletness
         assert |g'|>2;
         var dhc :| isDirectedHamiltonianCircuit(g, dhc);
 
-        // directedHamiltonianCircuitProperty_lemma(g, dhc);
         assert forall i :: 0<i<|g| ==> g[dhc[i-1]][dhc[i]] && g[dhc[|g|-1]][dhc[0]];
 
         var dhc_eq := circuit_equivalence(g, g', dhc);
-
-        // var dhc_uEq := circuit_equivalence(g, g', dhc);
-        // circuit_equivalent_lemma(g, g', dhc, dhc_uEq);
-
-        // assert forall i :: 0<i<|g| ==> (g[dhc[i-1]][dhc[i]] ==> g'[dhc[i-1]+|g|][dhc[i]+|g|*2]);
-        // assert forall i :: 0<i<|g| ==> (g[dhc[i-1]][dhc[i]] ==> g'[dhc[i-1]+|g|][dhc[i]+|g|*2]);
-        // assert g[dhc[|g|-1]][dhc[0]] ==> g'[dhc[|g|-1]+|g|][dhc[0]+|g|*2];
         
     }
-
-    // ghost predicate circuit_equivalent(g: Graph, g': Graph, circuit: seq<nat>, circuit': seq<nat>)
-    //     requires validGraph(g)
-    //     requires |g|>2
-    //     requires isDirectedHamiltonianCircuit(g, circuit)
-    //     requires g' == directed_to_undirected_graph(g)
-    //     // ensures forall i :: (0<=i<|circuit'| && i % 3 ==1)  ==> circuit'[i] == circuit[(i-1)/3]
-    // {
-    //     |circuit'|==|g|*3
-    //     &&
-    //     (
-    //         forall i :: 0<=i<|g| ==>    //giving the index of the original node i, the index of the same node in circuit': f(i)=3i+1
-    //         (
-    //             circuit'[i*3]==circuit[i]+|g|*2 //in node
-    //             &&
-    //             circuit'[i*3+1]==circuit[i] //central (original) node
-    //             &&
-    //             circuit'[i*3+2]==circuit[i]+|g| //out node
-    //         )
-    //     )
-    // }
-
-    // lemma circuit_equivalent_aux1_lemma(g: Graph, g': Graph, circuit: seq<nat>, circuit': seq<nat>)
-    //     requires validGraph(g)
-    //     requires |g|>2
-    //     requires isDirectedHamiltonianCircuit(g, circuit)
-    //     requires g' == directed_to_undirected_graph(g)
-    //     requires circuit_equivalent(g, g', circuit, circuit')
-    //     ensures forall i :: 0<=i<|circuit'| ==> circuit'[i]<|g'|
-    // {
-    //     forall i | 0<=i<|circuit'|
-    //     {
-    //         circuit_equivalent_aux1_local_lemma(g, g', circuit, circuit', i);
-    //     }
-    // }
-
-    // lemma circuit_equivalent_aux1_local_lemma(g: Graph, g': Graph, circuit: seq<nat>, circuit': seq<nat>, i: int)
-    //     requires validGraph(g)
-    //     requires |g|>2
-    //     requires isDirectedHamiltonianCircuit(g, circuit)
-    //     requires g' == directed_to_undirected_graph(g)
-    //     requires circuit_equivalent(g, g', circuit, circuit')
-    //     requires 0<=i<|circuit'|
-    //     ensures circuit'[i]<|g'|
-    // {
-    //     assert circuit'[i*3]==circuit[i]+|g|*2;
-    //     assert circuit'[i*3+1]==circuit[i];
-    //     assert circuit'[i*3+2]==circuit[i]+|g|;
-    // }
-
-    // lemma circuit_equivalent_lemma(g: Graph, g': Graph, circuit: seq<nat>, circuit': seq<nat>)
-    //     requires validGraph(g)
-    //     requires |g|>2
-    //     requires isDirectedHamiltonianCircuit(g, circuit)
-    //     requires g' == directed_to_undirected_graph(g)
-    //     requires circuit_equivalent(g, g', circuit, circuit')
-    //     ensures isUndirectedHamiltonianCircuit(g', circuit')
-    // {
-    //     if !isUndirectedHamiltonianCircuit(g', circuit')
-    //     {
-    //         reveal circuit_equivalent(g, g', circuit, circuit');
-    //         directedHamiltonianCircuitProperty_lemma(g, circuit);
-    //         assert forall i :: 0<i<|g| ==> g[circuit[i-1]][circuit[i]]; //property_lemma definition
-    //         assert forall i :: 0<=i<|g| ==> circuit'[i*3+1]==circuit[i] && circuit'[i*3]==circuit[i]+|g|*2 && circuit'[i*3+2]==circuit[i]+|g|;  //equivalence property
-    //         assert forall i :: 0<=i<|g| ==> 0<=circuit[i]<|g|;
-    //         assert forall i :: 0<=i<|g| ==> g'[circuit'[i*3+1]][circuit'[i*3]];
-    //     }
-    // }
 
     //returns the directed circuit's undirected equivalence
     ghost function circuit_equivalence(g: Graph, g': Graph, circuit: seq<nat>): seq<nat>
@@ -124,11 +50,23 @@ module ReductionCompletness
         requires g' == directed_to_undirected_graph(g)
         ensures isUndirectedHamiltonianCircuit(g', circuit_equivalence(g, g', circuit))
     {
-        circuit_equivalence_connectivity_lemma(g, g', circuit, |g|-1);
-        circuit_equivalence_(g, g', circuit, |g|-1)
+        var ce := circuit_equivalence_(g, g', circuit, |g|-1).0;
+        assert ce == circuit_equivalence_(g, g', circuit, |g|-1).0;   //sus muertos
+        assert UniqueElements(ce) by {circuit_equivalence_no_duplicates_lemma(g, g', circuit, |g|-1);}
+        aux_lemma(ce);
+        assert forall i :: 0<=i<|g'| ==> !(exists j :: 0<=j<|g'| && j!=i && ce[i]==ce[j]);  //ESTO: no hay elementos repetidos
+        ce
+        // forall j :: 0<=j<|circuit'| ==> !(exists r :: 0<=r<|circuit'| && j!=r && circuit'[j]==circuit'[r])
     }
 
-    ghost function circuit_equivalence_(g: Graph, g': Graph, circuit: seq<nat>, i: int): seq<nat>
+    /**
+    0: circuit equivalent
+    1-3 for verification purposes: partial correctness (no duplicates)
+        1: all original nodes
+        2: all out nodes
+        3: all in nodes
+     */
+    ghost function circuit_equivalence_(g: Graph, g': Graph, circuit: seq<nat>, i: int): (seq<nat>, seq<nat>, seq<nat>, seq<nat>)
         requires validGraph(g)
         requires |g|>2
         requires isDirectedHamiltonianCircuit(g, circuit)
@@ -136,140 +74,86 @@ module ReductionCompletness
         requires -1<=i<|circuit|
         decreases i
         //size relation
-        ensures |circuit_equivalence_(g, g', circuit, i)| == (i+1)*3
-        ensures |circuit_equivalence_(g, g', circuit, i)| % 3 == 0 //triplets
+        ensures |circuit_equivalence_(g, g', circuit, i).0| == (i+1)*3
+        ensures |circuit_equivalence_(g, g', circuit, i).0| % 3 == 0 //triplets
         // ensures |circuit_equivalence_(g, g', circuit, i)| == |circuit_equivalence_(g, g', circuit, i-1)|+3
         //central, in and out nodes position relation
         ensures forall j :: 0<=j<= i ==> 
         (
-            circuit_equivalence_(g, g', circuit, i)[3*j] == circuit[j]+|g|*2
+            circuit_equivalence_(g, g', circuit, i).0[3*j] == circuit[j]+|g|*2
             &&
-            circuit_equivalence_(g, g', circuit, i)[3*j+1] == circuit[j]
+            circuit_equivalence_(g, g', circuit, i).0[3*j+1] == circuit[j]
             &&
-            circuit_equivalence_(g, g', circuit, i)[3*j+2] == circuit[j]+|g|
+            circuit_equivalence_(g, g', circuit, i).0[3*j+2] == circuit[j]+|g|
         )
-        //reverse relation
-        ensures i>=0 ==>
-        (
-            var circuit' := circuit_equivalence_(g, g', circuit, i);
-            circuit'[|circuit'|-3] == circuit[(|circuit'|-3)/3]+|g|*2
-            &&
-            circuit'[|circuit'|-2] == circuit[((|circuit'|-2)-1)/3]
-            &&
-            circuit'[|circuit'|-1] == circuit[((|circuit'|-1)-2)/3]+|g|
-        )
-        // ensures forall j :: 0<=j<|circuit_equivalence_(g, g', circuit, i)| ==>
-        // (
-        //     (j % 3 == 0 ==> (circuit_equivalence_(g, g', circuit, i)[j] == circuit[(j)/3]+|g|*2))
-        //     &&
-        //     (j % 3 == 1 ==> (circuit_equivalence_(g, g', circuit, i)[j] == circuit[(j-1)/3]))
-        //     &&
-        //     (j % 3 == 2 ==> (circuit_equivalence_(g, g', circuit, i)[j] == circuit[(j-2)/3]+|g|))
-        // )
         //nodes boundaries
-        ensures forall j :: 0<j<|circuit_equivalence_(g, g', circuit, i)| ==> circuit_equivalence_(g, g', circuit, i)[j]<|g'|
+        ensures forall j :: 0<=j<|circuit_equivalence_(g, g', circuit, i).0| ==> circuit_equivalence_(g, g', circuit, i).0[j]<|g'|
         //connectivity
-        // ensures var circuit' := circuit_equivalence_(g, g', circuit, i);
-            // forall j :: 0<j<|circuit'| ==> g'[circuit'[j-1]][circuit'[j]]
+        ensures var circuit' := circuit_equivalence_(g, g', circuit, i).0;
+            forall j :: 0<j<|circuit'| ==> (g'[circuit'[j-1]][circuit'[j]] || g'[circuit'[j]][circuit'[j-1]])
+        //for partial correctness: no duplicates (working with 1, 2 & 3 sequences)
+        //sizes
+        ensures i>=0 ==> var a := circuit_equivalence_(g, g', circuit, i);
+            |a.1|==i+1 && |a.2|==i+1 && |a.3|==i+1
+        //contains
+        ensures forall j :: 0<=j<|circuit_equivalence_(g, g', circuit, i).1| ==> circuit_equivalence_(g, g', circuit, i).1[j]==circuit[j]
+        ensures forall j :: 0<=j<|circuit_equivalence_(g, g', circuit, i).2| ==> circuit_equivalence_(g, g', circuit, i).2[j] == circuit[j]+|g|
+        ensures forall j :: 0<=j<|circuit_equivalence_(g, g', circuit, i).3| ==> circuit_equivalence_(g, g', circuit, i).3[j] == circuit[j]+|g|*2
+        //unique elements (no duplicates)
+        ensures UniqueElements(circuit_equivalence_(g, g', circuit, i).1) && UniqueElements(circuit_equivalence_(g, g', circuit, i).2) && UniqueElements(circuit_equivalence_(g, g', circuit, i).3)
+        //no interdepenence: all elements in no overlapping ranges
+        ensures var a := circuit_equivalence_(g, g', circuit, i);
+            inRange(0, |g|, a.1) && inRange(|g|, |g|*2, a.2) && inRange(|g|*2, |g|*3, a.3)
     {
-        if i==-1 then [] else
+        if i==-1 then ([], [], [], []) else
             var circuit' := circuit_equivalence_(g, g', circuit, i-1);
-            var ret_circuit := circuit' + [circuit[i]+|g|*2] + [circuit[i]] + [circuit[i]+|g|];
-            // assert |ret_circuit| == |circuit'|+3;
-            // var i1, i2, i3 := |circuit'|, |circuit'|+1, |circuit'|+2;
-            // assert ret_circuit[i1] == circuit[(i1)/3]+|g|*2;
-            // assert ret_circuit[i2] == circuit[(i2-1)/3];
-            // assert ret_circuit[i3] == circuit[(i3-2)/3]+|g|;
-            ret_circuit
+            (circuit'.0 + [circuit[i]+|g|*2] + [circuit[i]] + [circuit[i]+|g|], circuit'.1+[circuit[i]], circuit'.2+[circuit[i]+|g|], circuit'.3+[circuit[i]+|g|*2])
     }
 
-    lemma circuit_equivalence_reverse_position_relation_lemma(g: Graph, g': Graph, circuit: seq<nat>, i: int)
+    //postcondition of circuit equivalence: circuit equivalent sequence is a permutation of 2nd + 3rd + 4th returning sequences
+    lemma circuit_equivalence_post_lemma(g: Graph, g': Graph, circuit: seq<nat>, i: int)
         requires validGraph(g)
         requires |g|>2
         requires isDirectedHamiltonianCircuit(g, circuit)
         requires g' == directed_to_undirected_graph(g)
         requires -1<=i<|circuit|
-        ensures var circuit' := circuit_equivalence_(g, g', circuit, i);
-            forall j :: 0<=j<|circuit'| ==>
-            (
-                (j % 3 == 0 ==> (circuit'[j] == circuit[(j)/3]+|g|*2))
-                &&
-                (j % 3 == 1 ==> (circuit'[j] == circuit[(j-1)/3]))
-                &&
-                (j % 3 == 2 ==> (circuit'[j] == circuit[(j-2)/3]+|g|))
-            )
-    {
-        if i>0
-        {
-            circuit_equivalence_reverse_position_relation_lemma(g, g', circuit, i-1);
-            var circuit1 := circuit_equivalence_(g, g', circuit, i-1);
-            var circuit2 := circuit_equivalence_(g, g', circuit, i);
-            assert circuit2 == circuit_equivalence_(g, g', circuit, i-1) + [circuit[i]+|g|*2] + [circuit[i]] + [circuit[i]+|g|];
-            assert forall j :: 0<=j<|circuit1| ==>
-            (
-                (j % 3 == 0 ==> (circuit1[j] == circuit[(j)/3]+|g|*2))
-                &&
-                (j % 3 == 1 ==> (circuit1[j] == circuit[(j-1)/3]))
-                &&
-                (j % 3 == 2 ==> (circuit1[j] == circuit[(j-2)/3]+|g|))
-            );
-            var j1, j2, j3 := |circuit2|-3, |circuit2|-2, |circuit2|-1;
-            assert j1%3==0 && j2%3==1 && j3%3==2;
-            // assert
-            // (
-            //     (j1 % 3 == 0 && (circuit1[j1] == circuit[(j1)/3]+|g|*2))
-            //     &&
-            //     (j2 % 3 == 1 && (circuit1[j2] == circuit[(j2-1)/3]))
-            //     &&
-            //     (j3 % 3 == 2 && (circuit1[j3] == circuit[(j3-2)/3]+|g|))
-            // );
-            assume forall j :: 0<=j<|circuit2| ==>
-            (
-                (j % 3 == 0 ==> (circuit2[j] == circuit[(j)/3]+|g|*2))
-                &&
-                (j % 3 == 1 ==> (circuit2[j] == circuit[(j-1)/3]))
-                &&
-                (j % 3 == 2 ==> (circuit2[j] == circuit[(j-2)/3]+|g|))
-            );
-        }
-    }
+        ensures multiset(circuit_equivalence_(g, g', circuit, i).0) == multiset(circuit_equivalence_(g, g', circuit, i).1) + multiset(circuit_equivalence_(g, g', circuit, i).2) + multiset(circuit_equivalence_(g, g', circuit, i).3)
+    {}
 
-    lemma circuit_equivalence_connectivity_lemma(g: Graph, g': Graph, circuit: seq<nat>, i: int)
+    /**
+    CRITICAL postcondition of circuit equivalence: circuit_equivalence has no duplicated values
+    (2nd + 3rd + 4th has no duplicated values) && (circuit equivalent is a permutation of 2nd + 3rd + 4th)
+        ||=> circuit equivalent has no duplicated values
+    Note: uses "permutation_property.dfy" file's module, see file and link at the top for further information
+    */
+    lemma circuit_equivalence_no_duplicates_lemma(g: Graph, g': Graph, circuit: seq<nat>, i: int)
         requires validGraph(g)
         requires |g|>2
         requires isDirectedHamiltonianCircuit(g, circuit)
         requires g' == directed_to_undirected_graph(g)
-        requires 0<=i<|circuit|
-        ensures var circuit' := circuit_equivalence_(g, g', circuit, i);
-            (forall j :: 0<j<|circuit'| ==> g'[circuit'[j-1]][circuit'[j]]) && g'[circuit'[|circuit'|-1]][circuit'[0]]
-    // {
-    //     var circuit' := circuit_equivalence_(g, g', circuit, i);
-    //     forall j | 0<j<|circuit'|
-    //     {
-    //         circuit_equivalence_connectivity_local_lemma(g, g', circuit, i, circuit', j);
-    //     }
-    // }
+        requires -1<=i<|circuit|
+        ensures UniqueElements(circuit_equivalence_(g, g', circuit, i).0)
+    {
+        var c' := circuit_equivalence_(g, g', circuit, i);
+        var s_aux := c'.1 + c'.2 + c'.3;
+        assert s_aux == c'.1 + c'.2 + c'.3;
+        assert UniqueElements(s_aux);
+        assert multiset(c'.0) == multiset(s_aux) by {circuit_equivalence_post_lemma(g, g', circuit, i);} //by is usefull here
+        assert |c'.0| == |s_aux|;
+        UniqueMultiSet(s_aux, c'.0);
+    }
 
-    // lemma circuit_equivalence_connectivity_local_lemma(g: Graph, g': Graph, circuit: seq<nat>, i: int, circuit': seq<nat>, j: int)
-    //     requires validGraph(g)
-    //     requires |g|>2
-    //     requires isDirectedHamiltonianCircuit(g, circuit)
-    //     requires g' == directed_to_undirected_graph(g)
-    //     requires 0<=i<|circuit|
-    //     requires circuit' == circuit_equivalence_(g, g', circuit, i)
-    //     requires 0<j<|circuit'|
-    //     ensures g'[circuit'[j-1]][circuit'[j]]
-    // {
-    //     if j%3==0
-    //     {
-    //         // assert circuit'[j] == circuit[j]+|g|*2;
-    //         assume g'[circuit'[j-1]][circuit'[j]];
-    //     }
-    //     if j%3==1
-    //     {assume g'[circuit'[j-1]][circuit'[j]];}
-    //     if j%3==2
-    //     {assume g'[circuit'[j-1]][circuit'[j]];}
-    // }
+    //trifling lemma for definition equivalences
+    lemma aux_lemma(s: seq<nat>)
+        requires UniqueElements(s)
+        ensures forall i :: 0<=i<|s| ==> !(exists j :: 0<=j<|s| && j!=i && s[i]==s[j])
+    {}
+
+    //auxiliar predicate
+    ghost predicate inRange(n1: int, n2: int, s:seq<nat>)
+    {
+        forall i :: 0<=i<|s| ==> n1<=s[i]<n2
+    }
 
     // Reduction to the left: undirectedHamiltonian(f(g)) ==> directedHamiltonian(g)
 
@@ -278,16 +162,5 @@ module ReductionCompletness
         requires undirectedHamiltonianCircuit(directed_to_undirected_graph(g))
         ensures directedHamiltonianCircuit(g)
     // {}
-
-
-    // ghost function directedHamiltonianCircuit_witness(g: Graph): seq<nat>
-    //     requires validGraph(g)
-    //     requires directedHamiltonianCircuit(g)
-    //     ensures isDirectedHamiltonianCircuit(g, (directedHamiltonianCircuit_witness(g)))
-
-    // ghost function undirectedHamiltonianCircuit_witness(g: Graph): seq<nat>
-    //     requires validUndirectedGraph(g)
-    //     requires undirectedHamiltonianCircuit(g)
-    //     ensures isUndirectedHamiltonianCircuit(g, (undirectedHamiltonianCircuit_witness(g)))
 
 }
