reduction_directedHamiltonianCircuit_to_hamiltonianCircuit/permutation_property.dfy
@@ -1,0 +1,82 @@
+module PermutationProperty
+{
+
+    /**
+    Question answered in stackoverflow:
+    https://stackoverflow.com/questions/77049958/problems-in-trying-to-prove-non-duplicate-element-sequence-in-dafny
+
+    1. If it is not case that all elements of sequence r are unique then there should exists indices m < n such that r[m] == r[n].
+    2. Next we try to pair up elements of sequence s (left) with element of sequence r (right) by equality.
+    3. To do that we find index ridx in r such r[ridx] equal to current element of s we are pairing.
+    4. Now if ridx happens to be n, then we can pair current element of s with r[m] as r[m] == r[n]
+    5. Effectively we are pairing up n distinct elements with n-1 elements.
+    6. We do some index shifting to convince dafny that we indeed pairing with n-1 elements on right side of matching.
+    7. By pigeonhole two elements of left should pair up with same element on right.
+    8. This means those two elements are equal but that is not possible as all elements are distinct on left side.
+    9. Our assumption is wrong and all elements on right side are distinct.
+    */
+
+    predicate UniqueElements(s: seq<int>)
+    {
+    forall i, j :: 0 <= i < j < |s| ==> s[i] != s[j]
+    }
+
+    lemma pigeonhole(m : int, n: int, f : int -> int)
+    requires 0 <= m < n
+    requires forall i :: 0 <= i < n ==> 0 <= f(i) < m
+    ensures exists j, k :: (0 <= j < k < n) && f(j) == f(k)
+    {
+    if m <= 0 {
+        assert 0 <= f(0) < 0;
+    }
+    else {
+        var i : int := 0;
+        while i < n
+        invariant forall k :: 0 <= k < i ==> 0 <= f(k) < m - 1
+        invariant i <= n
+        {
+        if f(i) == m-1 {
+            var j : int := i + 1;
+            while j < n
+            invariant forall k :: i < k < j ==> 0 <= f(k) < m - 1
+            {
+            if f(j) == m-1 { return; }
+                j := j + 1;
+            }
+            var g : int -> int := x => if x < i then f(x) else f(x+1);
+            pigeonhole(m-1, n-1, g);
+            return;
+        }
+        i := i + 1;
+        }
+        pigeonhole(m-1, n, f);
+    }
+    }
+
+
+    lemma UniqueMultiSet(s: seq<int>, r: seq<int>)
+    requires UniqueElements(s)
+    requires |s| == |r|
+    requires multiset(s) == multiset(r)
+    ensures UniqueElements(r)
+    {
+    assert |multiset(s)| == |multiset(r)|;
+    if !UniqueElements(r){
+        var m, n :| 0 <= m < n < |r| && r[m] == r[n];
+        forall idx | 0 <= idx < |s| ensures exists ridx :: 0 <= ridx < |r| && r[ridx] == s[idx]
+        {
+        assert s[idx] in multiset(r);
+        }
+        var f : int -> int :=
+        x => if 0 <= x < |s|
+            then
+                var idx :| 0 <= idx < |r| && r[idx] == s[x];
+                if idx < n then idx else if idx == n then m else idx - 1
+            else -1;
+        pigeonhole(|s|-1, |s|, f);
+        var k, l :| 0 <= k < l < |s| && f(k) == f(l);
+        assert s[k] == s[l];
+    }
+    }
+
+}
